Rework protocols

src/Protocol.v
@@ -27,12 +27,12 @@ Fixpoint tuple_to_hlist A (T : A) P n (t : tuple (P T) n)
   induction t; constructor; assumption.
 Defined.
 
-Inductive In_with_tail A : A -> list A -> list A -> Type :=
+Inductive In_with_tail A : A -> list A -> list A -> Prop :=
 | Here : forall hd tl, In_with_tail hd tl (hd :: tl)
 | Next : forall hd tl x xs, In_with_tail hd tl xs ->
                             In_with_tail hd tl (x :: xs).
 
-Section Protocol.
+Section Protocols.
 
   Context (sort : Type)
           (func : list sort -> sort -> Type)
@@ -49,62 +49,95 @@ Section Protocol.
   Notation "'term'" := (term func).
   Notation "'model'" := (model func predicate).
 
-  Variable Q : nat -> Type.
-  Variable q0 : Q 0.
+  Section Protocol.
 
-  Record transition n := mkTransition {
-      from : Q n;
-      to : Q (S n);
-      output : tuple (term message) n -> term message -> term message;
-      guard : tuple (term message) n -> term message -> term sbool
-  }.
+    Variable Q : nat -> Type.
+    Variable q0 : Q 0.
 
-  Variable transitions : forall n (q : Q n), list (transition n).
-  Variable transitions_from : forall n (q : Q n) t,
-                                In t (transitions q) -> t.(from) = q.
+    Record transition_ n (from : Q n) (to : Q (S n)) :=
+      mkTransition {
+          output : tuple (term message) n -> term message -> term message;
+          guard : tuple (term message) n -> term message -> term sbool
+        }.
 
-  Definition final n (q : Q n) : Prop := transitions q = [].
+    Variable transitions : forall n (q : Q n),
+                             list {q' : Q (S n) & transition_ q q'}.
 
-  Definition maximal n (t : transition n) : Prop :=
-    forall (is : tuple (term message) n) (i : term message),
-      t.(guard) is i = App ftrue h[].
+    Definition final_ n (q : Q n) : Prop := transitions q = [].
 
-  Definition has_max_transition n (q : Q n) (H : ~final q) : Prop :=
-    maximal (head H).
+    Definition maximal_transition n q q' (t : transition_ q q') : Prop :=
+      forall (is : tuple (term message) n) (i : term message),
+        t.(guard) is i = App ftrue h[].
 
-  Variable max_transition : forall n (q : Q n) (H : ~final q),
-                              has_max_transition H.
+    Definition has_max_transition n (q : Q n) (H : ~final_ q) : Prop :=
+      maximal_transition (projT2 (head H)).
 
-  Variable initial_knowledge : list (term message).
+  End Protocol.
 
-  Variable handles : forall n : nat,
-                       func (repeat message (n + length initial_knowledge))
-                            message.
+  Record protocol :=
+    mkProtocol {
+        Q : nat -> Type;
+        q0 : Q 0;
+        transition : forall n, Q n -> Q (S n) -> Type := @transition_ Q;
+        transitions : forall n (q : Q n),
+                        list {q' : Q (S n) & transition q q'};
+        final : forall n, Q n -> Prop := @final_ Q transitions;
+        max_transition : forall n (q : Q n) (H : ~final q),
+                           has_max_transition H;
+        initial_knowledge : list (term message);
+        handles : forall n : nat,
+                    func (repeat message (n + length initial_knowledge))
+                         message
+      }.
 
-  Inductive execution (m : model)
-  : forall n, Q n -> tuple (term message) n ->
-              tuple (term message) (n + length initial_knowledge)
+  Inductive execution (p : protocol)
+  : forall n, p.(Q) n -> tuple (term message) n ->
+              tuple (term message) (n + length p.(initial_knowledge))
               -> Type :=
-  | Initial : execution m q0 t[] (list_to_tuple initial_knowledge)
+  | Initial : execution p.(q0) t[] (list_to_tuple p.(initial_knowledge))
   | Transition :
-      forall n (q : Q n) (inputs : tuple (term message) n)
-             (knowledge : tuple (term message)
-                                (n + length initial_knowledge))
-             (t : transition n) (l : list (transition n)) q',
-        In_with_tail t l (transitions q) ->
-        t.(to) = q' ->
-        execution m q inputs knowledge ->
-        let new_input := (App (handles n)
+      forall n (q : p.(Q) n) inputs knowledge q' (t : transition q q'),
+        execution q inputs knowledge ->
+        let new_input := (App (p.(handles) n)
                               (tuple_to_hlist knowledge)) in
         let new_inputs := new_input t:: inputs in
         let new_knowledge :=
             t.(output) inputs new_input t:: knowledge in
-        m.(interp_term) (t.(guard) inputs new_input) =
-        m.(interp_term) (App ftrue h[]) ->
-        (forall (t' : transition n),
-           In t' l ->
-           m.(interp_term) (t.(guard) inputs new_input) <>
-           m.(interp_term) (App ftrue h[])) ->
-        execution m q' new_inputs new_knowledge.
+        execution q' new_inputs new_knowledge.
 
-End Protocol.
+  Inductive Execution (p : protocol) : Type :=
+  | exec : forall n (q : p.(Q) n) inputs knowledge
+                  (e : execution q inputs knowledge), Execution p.
+
+  Definition valid_exec (m : model) (p : protocol) (e : Execution p) : Prop.
+    destruct e as [n q inputs knowledge e].
+    induction e.
+    exact True.
+    exact (exists t_ l,
+             In_with_tail t_ l (transitions q) /\
+             (exists H : q' = projT1 t_,
+                projT2 t_ = eq_rect q' (transition _) t (projT1 t_) H) /\
+             m.(interp_term) (t.(guard) inputs new_input) =
+             m.(interp_term) (App ftrue h[]) /\
+             (forall t'_, In t'_ l ->
+                          let t' := projT2 t'_ in
+                          m.(interp_term) (t'.(guard) inputs new_input) <>
+                          m.(interp_term) (App ftrue h[]))).
+  Defined.
+
+  Definition final_exec (p : protocol) (e : Execution p) : Prop :=
+    match e with
+      | @exec _ _ q _ _ _ => final q
+    end.
+
+  Theorem exec_final_valid_unique :
+    forall (m : model) (p : protocol) (e e' : Execution p),
+      final_exec e -> final_exec e' -> valid_exec m e -> valid_exec m e' ->
+      e = e'.
+    intros m p e e' Hfe Hfe' Hve Hve'.
+  Admitted.  (* TODO *)
+
+  (* Existence of a final valid execution requires at least decidability
+  over domain bool *)
+
+End Protocols.
